# Activity 3.1 - Regular languages

Reference for math symbols:
https://www.overleaf.com/learn/latex/List_of_Greek_letters_and_math_symbols

## Names:
- Emilia Salazar Leipen
- Fernanda Osorio
- Ian Holender 


## Exercises:

1. Give a recursive definition of the set of strings over $\{a, b\}$ that
    contain at least one $b$ and have an even number of $a$’s before the
    first $b$.
    For example: $aab$, $bab$ and $aaaabbabababa$ are in the set,
    but $abb$, $aaab$ and $aa$ are not

    
    <span style="color:red;">_**SOLUTION:**_</span>

    
    **I. Basis:** $b \in S$

    **II. Recursive Step**: If $u \in S$ then $uab \in S$. (According to "at least one $b$ and have an even number of $a$’s before the first $b$") 
    If $ uaa \in S$ then $uaab \in S$

    **III. Closure**: A string $u \in S$ only if it can be obtained from the basis using a finite number of applications of the recursive step.


2. Let $X = \{aa, bb\}$ and $Y = \{\lambda, b, ab\}$.

    a. List the strings in set $XY$

    #|string|#|string|#|string
    -|-|-|-|-|-
    aa  || aab || aaab|| 
    bb  || bbb || bbab

    b. How many strings of length 6 are there in $X^*$?
    
    $X=\{aa, bb\}$

    $XX=$

    $XXX=\{aa, bb\}\{aa, bb\}\{aa, bb\}$

    


    - aaaaaa
    - aaaabb
    - aabbaa
    - aabbbb
    - bbaaaa
    - bbaabb
    - bbbbaa
    - bbbbbb
    $$2^3=8$$

    There are 8 stringth with length 6 in $X^*$.

   

    c. List the strings in set $Y^*$ of length three or less

    
    #|string|#|string|#|string
    -|-|-|-|-|-
    $\lambda$ || $\lambda$ b|| $\lambda$ ab|| 
    bb || abb|| aabb ||
    bab ||  || ||

    

    d. List the strings in set $X^* Y^*$ of length four or less

    $ xx = \{ aa, bb, aaaa, bbbb, aabb, bbaa \} $

    The sets that will be taken into consideration are:

    $ = \{ aa, bb, aaaa, bbbb, aabb, bbaa \} $

   $ yyyy =  \newline \{ \lambda , b, ab \} \newline \{ \lambda , b, ab \} \newline \{ \lambda , b, ab \} \newline \{ \lambda , b, ab \} \newline  $ 

   $ = \{ \lambda , b, ab, bb, bab, abb, abab, bbb, bbab, bbabab, abbb, abbab, ababab, bbbb, babb \}$

   The sets that will be taken into consideration are:

   $ = \{ \lambda, b, ab, bb, bab, abb, abab, bbb, bbab, abbb, bbbb, babb \}$

X|Y|
-|-|
$\lambda$|$\lambda$|
aa|b
bb|ab
aabb|bb
bbaa|bab
aaaa|abb
bbbb|abab
| |bbb
| |bbab
| |babb
| |bbbb
| |abbb


$X^* Y^*$
| # | String |
|---|--------|
| 1 | λ      |
| 2 | b      |
| 3 | ab     |
| 4 | bab    |
| 5 | abb    |
| 6 | abab   |
| 7 | babb   |
| 8 | abbb   |
| 9 | aa     |
|10 | bb     |
|11 | bbb    |
|12 | bbab   |
|13 | bbbb   |
|14 | aab    |
|15 | aaab   |
|16 | aabb   |
|17 | bbaa   |
|18 | aaaa   |




3. Give a recursive definition of the set $\{ a^ib^j | 0 ≤ i ≤ j ≤ 2i\}$

    _**SOLUTION:**_

**I. Basis:** $\lambda \in L$

**II. Recursive Step**:
If $u \in L$ then $aub \in L$ and $aub^2 \in L$

If the string u belongs in L, then aub satisfies the condition of the set, and aub^2 also satisfies the condition of the set because while keeping the i constant, the j is doubled, stisfying the condition that the number of b´s will not be more than twice the number of a´s.

  **III. Closure**: A string $u \in L$ only if it can be obtained from the basis using a finite number of applications of the recursive step.



4. Let $L$ be the set of strings over $\{a, b\}$ generated by the recursive
   definition

    **I. Basis:** $b \in L$

    **II. Recursive Step**: If $u \in L$ then $ub \in L$, $uab \in L$, $uba \in
    L$ and $bua \in L$

    **III. Closure**: A string $u \in L$ only if it can be obtained from the
    basis using a finite number of applications of the recursive step.

    **a.** List the elements in the sets $L_0, L_1, L_2$

   $L_0={b} \rightarrow $ base case

   $L_1={bb, bab, bba} \rightarrow $ apply recursive step to $L_0$ 
   - $u=b$
   - $ub \rightarrow bb$
   - $uab \rightarrow bab$
   - $uba \rightarrow bba$
    - $bua \rightarrow bba$
   

   $L_2={bbb, bbab, bbba, babb, babab, babba, bbaab, bbaba, bbbaa}  \rightarrow $ apply recursive step to $L_1$ 
   
   - $u=bb$
     -  $ub \rightarrow bbb$
     - $uab \rightarrow bbab$
     - $uba \rightarrow bbba$
     - $bua \rightarrow bbba$

    - $u=bab$
        - $ub \rightarrow babb$
         - $uab \rightarrow babab$
         - $uba \rightarrow babba$
         - $bua \rightarrow bbaba$

    - $u=bba$
         - $ub \rightarrow bbab$
         - $uab \rightarrow bbaab$
         - $uba \rightarrow bbaba$
         - $bua \rightarrow bbbaa$


    **b.** Is the string $bbaaba$ in $L$? If so, trace how it is produced.
    If not, explain why not.
    The string does not belong in L, we can infere this by trying to trace the string which will be impossible, as well as by seeing the recurssive the way the a's and the b's are placed in the string, which do not match the conditions of the set.




    **c.** Is the string $bbaaaabb$ in $L$? If so, trace how it is produced.
    If not, explain why not

Yes the sttring belongs in L:

- $b $
- $bba$ 
    - $bua \rightarrow  u=b$
- $bbab$
    - $ub \rightarrow  u=bba$
- $bbaaab$
    -  $uab \rightarrow  u=bbab$
- $bbaaaabb$
    -  $ub \rightarrow  u=bbaaab$


5. Prove, using induction on the length of a string, that $(w^R)^R = w$ for all
   string $w \in \Sigma$

    <span style="color:red;">_**SOLUTION:**_</span>

    **I. Basis:**  $ w = \lambda $ (empty string). Given that the reverse of an empty string is also an empty string, we have that $ (w^R)^R = (\lambda^R)^R = \lambda ^R  = \lambda = w$. (Hypothesis)

    **II. Inductive Step:**  Assuming that the hypothesis holds for any string of lenght $ n $ or less, we have to prove that it holds for any string of lenght $ n+1 $.
        i.e.  $(w^R)^R = w \Leftrightarrow |w| ≤ n$

    In order to prove the hypothesis. Let $w = ax$ where $x \in \Sigma^*$ (including zero) is a string of lenght $n$ or less; and $a \in \Sigma$ represents a character. 

    *Inductive Hypothesis:*  $(x^R)^R = x \\(\Leftrightarrow |x| ≤ n)$  

    Using the induction hypothesis we can reverse the string $w$. 

    $$ w^R = (xa)^R = a^R x^R = ax^R $$
    $$ (w^R)^R = (ax^R)^R = (x^R)^R a^R = x a = w $$

    Consequently proving our hypothesis and showing that $(w^R)^R = w (\Leftrightarrow |x| ≤ n)$ using the induction hypothesis.




